flip library and recover lazy_eager_coin.v

theories/examples/lazy_eager_coin.v
@@ -4,6 +4,7 @@ From self.prob_lang Require Import notation proofmode primitive_laws spec_rules.
 From self.logrel Require Import model rel_rules rel_tactics.
 From self.typing Require Import soundness.
 From self.prelude Require Import base.
+From self.examples.lib Require Import flip.
 Set Default Proof Using "Type*".
 
 (** The lazy/eager coins, without tapes *)
@@ -11,24 +12,24 @@ Definition lazy : expr :=
   let: "s" := ref NONEV in
   λ: <>,
     match: !"s" with
-    | NONE => let: "b" := flip #() in
+    | NONE => let: "b" := flip in
               "s" <- SOME "b" ;;
               "b"
     | SOME "b" => "b"
     end.
 
 Definition eager : expr :=
-  let: "b" := flip #() in
+  let: "b" := flip in
   λ: <>, "b".
 
 (** An intetermedaite version of [lazy] that uses a tape to allow presampling
     bits during the proof *)
 Definition lazy_with_tape : expr :=
-  let: "α" := alloc #1%nat in
+  let: "α" := allocB in
   let: "s" := ref NONEV in
   λ: <>,
     match: !"s" with
-    | NONE => let: "b" := flip "α" in
+    | NONE => let: "b" := flipL "α" in
               "s" <- SOME "b" ;;
               "b"
     | SOME "b" => "b"
@@ -41,17 +42,17 @@ Section logical_ref.
 
   (** lazy << lazy_with_tape << eager *)
   Lemma lazy_lazy_with_tape_rel :
-    ⊢ REL lazy << lazy_with_tape : () → lrel_nat.
+    ⊢ REL lazy << lazy_with_tape : () → lrel_bool.
   Proof.
     rewrite /lazy /lazy_with_tape.
     rel_alloc_l l as "Hl".
     rel_pures_l.
-    rel_alloctape_r α as "Hα".
+    rel_allocBtape_r α as "Hα".
     rel_pures_r.
     rel_alloc_r l' as "Hl'".
     rel_pures_r.
-    set (P := (α ↪ₛ (1%nat; []) ∗ (l ↦ NONEV ∗ l' ↦ₛ NONEV ∨
-               ∃ (b : fin 2), l ↦ SOMEV #b ∗ l' ↦ₛ SOMEV #b))%I).
+    set (P := (α ↪ₛB [] ∗ (l ↦ NONEV ∗ l' ↦ₛ NONEV ∨
+               ∃ b : bool, l ↦ SOMEV #b ∗ l' ↦ₛ SOMEV #b))%I).
     iApply (refines_na_alloc P coinN).
     iSplitL.
     { iFrame. iLeft. iFrame. }
@@ -64,9 +65,9 @@ Section logical_ref.
     iIntros "[(Hα & [[Hl Hl'] | >[%b [Hl Hl']]]) Hclose]".
     - rel_load_l. rel_pures_l.
       rel_load_r. rel_pures_r.
-      rel_bind_l (rand _ from _)%E.
-      rel_bind_r (rand _ from _)%E.
-      iApply (refines_couple_rands_r with "[-$Hα]").
+      rel_bind_l flip.
+      rel_bind_r (flipL _)%E.
+      iApply (refines_couple_flip_flipL with "[-$Hα]").
       iIntros (b) "Hα /=".
       rel_pures_l. rel_store_l. rel_pures_l.
       rel_pures_r. rel_store_r. rel_pures_r.
@@ -81,16 +82,17 @@ Section logical_ref.
   Qed.
 
   Lemma lazy_with_tape_eager_rel :
-    ⊢ REL lazy_with_tape << eager : () → lrel_nat.
+    ⊢ REL lazy_with_tape << eager : () → lrel_bool.
   Proof.
     rewrite /lazy_with_tape /eager.
-    rel_alloctape_l α as "Hα". rel_pures_l.
-    rel_bind_r (rand _ from _)%E.
-    iApply (refines_couple_tape_rand with "[$Hα]"); [done|].
+    rel_allocBtape_l α as "Hα".
+    rel_pures_l.
+    rel_bind_r flip.
+    iApply (refines_couple_tape_flip with "[$Hα]"); [solve_ndisj|done|].
     iIntros (b) "Hα /=".
     rel_pures_r.
     rel_alloc_l l as "Hl". rel_pures_l.
-    set (P := ((α ↪ (1; [b]) ∗ l ↦ NONEV) ∨ (l ↦ SOMEV #b))%I).
+    set (P := ((α ↪B [b] ∗ l ↦ NONEV) ∨ (l ↦ SOMEV #b))%I).
     iApply (refines_na_alloc P coinN).
     iSplitL.
     { iModIntro. iLeft. iFrame. }
@@ -101,7 +103,7 @@ Section logical_ref.
     iApply (refines_na_inv with "[$Hinv]"); [done|].
     iIntros "[[[Hα Hl] | Hl] Hclose]".
     - rel_load_l. rel_pures_l.
-      rel_rand_l. rel_pures_l.
+      rel_flipL_l. rel_pures_l.
       rel_store_l. rel_pures_l.
       iApply (refines_na_close with "[- $Hclose]").
       iSplitL; [|rel_values].
@@ -114,16 +116,16 @@ Section logical_ref.
 
   (** eager << lazy_with_tape << lazy *)
   Lemma eager_lazy_with_tape_rel :
-    ⊢ REL eager << lazy_with_tape : () → lrel_nat.
+    ⊢ REL eager << lazy_with_tape : () → lrel_bool.
   Proof.
     rewrite /lazy_with_tape /eager.
-    rel_alloctape_r α as "Hα". rel_pures_r.
-    rel_bind_l (rand _ from _ )%E.
-    iApply (refines_couple_rand_tape with "[$Hα]").
+    rel_allocBtape_r α as "Hα". rel_pures_r.
+    rel_bind_l flip.
+    iApply (refines_couple_flip_tape with "[$Hα]").
     iIntros (b) "Hα /=".
     rel_pures_r.
     rel_alloc_r l as "Hl". rel_pures_r.
-    set (P := ((α ↪ₛ (1; [b]) ∗ l ↦ₛ NONEV) ∨ (l ↦ₛ SOMEV #b))%I).
+    set (P := ((α ↪ₛB [b] ∗ l ↦ₛ NONEV) ∨ (l ↦ₛ SOMEV #b))%I).
     iApply (refines_na_alloc P coinN).
     iSplitL.
     { iModIntro. iLeft. iFrame. }
@@ -134,7 +136,7 @@ Section logical_ref.
     iApply (refines_na_inv with "[$Hinv]"); [done|].
     iIntros "[[>[Hα Hl] | >Hl] Hclose]".
     - rel_load_r. rel_pures_r.
-      rel_rand_r. rel_pures_r.
+      rel_flipL_r. rel_pures_r.
       rel_store_r. rel_pures_r.
       iApply (refines_na_close with "[- $Hclose]").
       iSplitL; [|rel_values].
@@ -146,14 +148,14 @@ Section logical_ref.
   Qed.
 
   Lemma lazy_with_tape_lazy_rel :
-    ⊢ REL lazy_with_tape << lazy : () → lrel_nat.
+    ⊢ REL lazy_with_tape << lazy : () → lrel_bool.
   Proof.
     rewrite /lazy /lazy_with_tape.
     rel_alloc_r l' as "Hl'". rel_pures_l.
-    rel_alloctape_l α as "Hα". rel_pures_l.
+    rel_allocBtape_l α as "Hα". rel_pures_l.
     rel_alloc_l l as "Hl". rel_pures_l.
-    set (P := (α ↪ (1; []) ∗ (l ↦ NONEV ∗ l' ↦ₛ NONEV ∨
-               ∃ (b: fin 2), l ↦ SOMEV #b ∗ l' ↦ₛ SOMEV #b))%I).
+    set (P := (α ↪B [] ∗ (l ↦ NONEV ∗ l' ↦ₛ NONEV ∨
+               ∃ (b : bool), l ↦ SOMEV #b ∗ l' ↦ₛ SOMEV #b))%I).
     iApply (refines_na_alloc P coinN).
     iSplitL.
     { iFrame. iLeft. iFrame. }
@@ -166,9 +168,9 @@ Section logical_ref.
     iIntros "[(Hα & [[Hl Hl'] | >[%b [Hl Hl']]]) Hclose]".
     - rel_load_l. rel_pures_l.
       rel_load_r. rel_pures_r.
-      rel_bind_l (rand _ from _)%E.
-      rel_bind_r (rand _ from _)%E.
-      iApply (refines_couple_rands_l with "[-$Hα]").
+      rel_bind_l (flipL _)%E.
+      rel_bind_r flip.
+      iApply (refines_couple_flipL_flip with "[-$Hα]"); [solve_ndisj|].
       iIntros (b) "Hα /=".
       rel_pures_l. rel_store_l. rel_pures_l.
       rel_pures_r. rel_store_r. rel_pures_r.
@@ -185,7 +187,7 @@ Section logical_ref.
 End logical_ref.
 
 Theorem lazy_eager_refinement :
-  ∅ ⊨ lazy ≤ctx≤ eager : () → TNat.
+  ∅ ⊨ lazy ≤ctx≤ eager : () → TBool.
 Proof.
   eapply ctx_refines_transitive.
   - eapply (refines_sound prelogrelΣ).
@@ -195,7 +197,7 @@ Proof.
 Qed.
 
 Theorem eager_lazy_refinement :
-  ∅ ⊨ eager ≤ctx≤ lazy : () → TNat.
+  ∅ ⊨ eager ≤ctx≤ lazy : () → TBool.
 Proof.
   eapply ctx_refines_transitive.
   - eapply (refines_sound prelogrelΣ).
@@ -205,7 +207,7 @@ Proof.
 Qed.
 
 Theorem eager_lazy_equiv :
-  ∅ ⊨ lazy =ctx= eager : () → TNat.
+  ∅ ⊨ lazy =ctx= eager : () → TBool.
 Proof.
   split.
   - apply lazy_eager_refinement.
